More MoreDep.v

test-suite/MoreDep.v
@@ -53,14 +53,14 @@ Equations typeDenote (t : type) : Set :=
 typeDenote Nat := nat;
 typeDenote Bool := bool;
 typeDenote (Prod t1 t2) := (typeDenote t1 * typeDenote t2)%type.
-(*
+
 Equations expDenote t (e : exp t) : typeDenote t :=
 expDenote _ (NConst n) := n;
 expDenote _ (Plus e1 e2) := expDenote e1 + expDenote e2;
-expDenote _ (Eq e1 e2) <= eq_nat_dec (expDenote e1) (expDenote e2) => {
+expDenote _ (Eq e1 e2) (* FIXME <= eq_nat_dec (expDenote e1) (expDenote e2) => {
   | left _ := true;
   | right _ := false
-};
+}; *) := beq_nat (expDenote e1) (expDenote e2);
 expDenote _ (BConst b) := b;
 expDenote _ (And e1 e2) := expDenote e1 && expDenote e2;
 expDenote _ (If e e1 e2) <= expDenote e => {
@@ -70,4 +70,233 @@ expDenote _ (If e e1 e2) <= expDenote e => {
 expDenote _ (Pair _ _ e1 e2) := (expDenote e1, expDenote e2);
 expDenote _ (Fst _ _ e) := fst (expDenote e);
 expDenote _ (Snd _ _ e) := snd (expDenote e).
+Next Obligation.
+  induction e; constructor; auto.
+  destruct (expDenote e1); constructor; auto.
+Defined.
+
+(* FIXME
+Equations pairOutType (t : type) : Set :=
+pairOutType (Prod t1 t2) := option (exp t1 * exp t2);
+pairOutType _ := option unit.
 *)
+
+Definition pairOutType (t : type) := option (match t with
+                                               | Prod t1 t2 => exp t1 * exp t2
+                                               | _ => unit
+                                             end).
+
+Equations pairOut t (e : exp t) : pairOutType t :=
+pairOut _ (Pair _ _ e1 e2) => Some (e1, e2);
+pairOut _ _ => None.
+
+(* FIXME
+Equations cfold t (e : exp t) : exp t :=
+cfold _ (NConst n) := NConst n;
+cfold _ (Plus e1 e2) <= (cfold e1, cfold e2) => {
+  | pair (NConst n1) (NConst n2) := NConst (n1 + n2);
+  | pair e1' e2' := Plus e1' e2'
+};
+cfold _ (Eq e1 e2) <= (cfold e1, cfold e2) => {
+  | pair (NConst n1) (NConst n2) <= eq_nat_dec n1 n2 => {
+    | left _ := BConst true;
+    | right _ := BConst false
+  };
+  | pair e1' e2' => Eq e1' e2'
+};
+cfold _ (BConst b) := BConst b;
+cfold _ (And e1 e2) <= (cfold e1, cfold e2) => {
+  | pair (BConst b1) (BConst b2) := BConst (b1 && b2);
+  | pair e1' e2' := And e1' e2'
+};
+cfold _ (If _ e e1 e2) <= cfold e => {
+  | BConst true := cfold e1;
+  | BConst false := cfold e2;
+  | e' := If e' (cfold e1) (cfold e2)
+};
+cfold _ (Pair e1 e2) := Pair (cfold e1) (cfold e2);
+cfold _ (Fst e) <= cfold e => {
+  | e' <= pairOut e' => {
+    | Some p := fst p;
+    | None := Fst e'
+  }
+};
+cfold _ (Snd e) <= cfold e => {
+  | e' <= pairOut e' => {
+    | Some p := snd p;
+    | None := Snd e'
+  }
+}.
+*)
+
+Inductive color : Set := Red | Black.
+
+Inductive rbtree : color -> nat -> Set :=
+| Leaf : rbtree Black 0
+| RedNode : forall n, rbtree Black n -> nat -> rbtree Black n -> rbtree Red n
+| BlackNode : forall c1 c2 n, rbtree c1 n -> nat -> rbtree c2 n -> rbtree Black (S n).
+
+Require Import Max Min Omega.
+
+Section depth.
+  Variable f : nat -> nat -> nat.
+
+  Equations depth c n (t : rbtree c n) : nat :=
+  depth _ _  Leaf := 0;
+  depth _ _ (RedNode _ t1 _ t2) := S (f (depth t1) (depth t2));
+  depth _ _ (BlackNode _ _ _ t1 _ t2) := S (f (depth t1) (depth t2)).
+End depth.
+
+Theorem depth_min : forall c n (t : rbtree c n), depth min t >= n.
+Proof.
+  intros. funelim (depth Nat.min t); auto;
+  match goal with
+  | [ |- context[min ?X ?Y] ] =>
+      let H := fresh in destruct (min_dec X Y) as [H|H]; rewrite H
+  end; omega.
+Qed.
+
+Lemma depth_max' : forall c n (t : rbtree c n), match c with
+                                                  | Red => depth max t <= 2 * n + 1
+                                                  | Black => depth max t <= 2 * n
+                                                end.
+Proof.
+  intros; funelim (depth Nat.max t); auto;
+  match goal with
+  | [ |- context[max ?X ?Y] ] =>
+      let H := fresh in destruct (max_dec X Y) as [H|H]; rewrite H
+  end;
+  repeat match goal with
+  | [ H : context[match ?C with Red => _ | Black => _ end] |- _ ] =>
+      destruct C
+  end; omega.
+Qed.
+
+Theorem depth_max : forall c n (t : rbtree c n), depth max t <= 2 * n + 1.
+Proof.
+  intros; generalize (depth_max' t); destruct c; omega.
+Qed.
+
+Theorem balanced : forall c n (t : rbtree c n), 2 * depth min t + 1 >= depth max t.
+Proof.
+  intros; generalize (depth_min t); generalize (depth_max t); omega.
+Qed.
+
+Inductive rtree : nat -> Set :=
+| RedNode' : forall c1 c2 n, rbtree c1 n -> nat -> rbtree c2 n -> rtree n.
+
+Section present.
+  Variable x : nat.
+
+  Equations present c n (t : rbtree c n) : Prop :=
+  present _ _ Leaf := False;
+  present _ _ (RedNode _ a y b) := present a \/ x = y \/ present b;
+  present _ _ (BlackNode _ _ _ a y b) := present a \/ x = y \/ present b.
+
+  Equations rpresent n (t : rtree n) : Prop :=
+  rpresent _ (RedNode' _ _ _ a y b) => present a \/ x = y \/ present b.
+End present.
+
+Notation "{< x >}" := (existT _ _ x).
+
+(* No need for convoy pattern! *)
+Equations balance1 n (a : rtree n) (data : nat) c2 (b : rbtree c2 n) : {c : color & rbtree c (S n)} :=
+balance1 _ (RedNode' _ c0 _ t1 y t2) data _ d <= t1 => {
+  | RedNode _ a x b := {<RedNode (BlackNode a x b) y (BlackNode t2 data d)>};
+  | _ <= t2 => {
+    | RedNode _ b x c := {<RedNode (BlackNode t1 y b) x (BlackNode c data d)>};
+    | b := {<BlackNode (RedNode t1 y (* ? b *) t2) data d>}
+  }
+}.
+
+Equations balance2 n (a : rtree n) (data : nat) c2 (b : rbtree c2 n) : {c : color & rbtree c (S n)} :=
+balance2 _ (RedNode' _ c0 _ t1 z t2) data _ a <= t1 => {
+  | RedNode _ b y c := {<RedNode (BlackNode a data b) y (BlackNode c z t2)>};
+  | _ <= t2 => {
+    | RedNode _ c z' d := {<RedNode (BlackNode a data t1) z (BlackNode c z' d)>};
+    | _ := {<BlackNode a data (RedNode t1 z t2)>}
+  }
+}.
+
+Section insert.
+  Variable x : nat.
+
+  Equations insResult (c : color) (n : nat) : Set :=
+  insResult Red n := rtree n;
+  insResult Black n := {c' : color & rbtree c' n}.
+
+  Equations ins c n (t : rbtree c n) : insResult c n :=
+  ins _ _ Leaf := {< RedNode Leaf x Leaf >};
+  ins _ _ (RedNode _ a y b) <= le_lt_dec x y => {
+    | left _ := RedNode' (projT2 (ins a)) y b;
+    | right _ := RedNode' a y (projT2 (ins b))
+  };
+  ins _ _ (BlackNode c1 c2 _ a y b) <= le_lt_dec x y => {
+    | left _ <= c1 => {
+      | Red := balance1 (ins a) y b;
+      | Black := {<BlackNode (projT2 (ins a)) y b>}
+    };
+    | right _ <= c2 => {
+      | Red := balance2 (ins b) y a;
+      | Black := {< BlackNode a y (projT2 (ins b))>}
+    }
+  }.
+
+  Equations insertResult (c : color) (n : nat) : Set :=
+  insertResult Red n := rbtree Black (S n);
+  insertResult Black n := {c' : color & rbtree c' n}.
+
+  Equations makeRbtree c n (r : insResult c n) : insertResult c n :=
+  makeRbtree Red _ (RedNode' _ _ _ a x b) := BlackNode a x b;
+  makeRbtree Black _ r := r.
+  Next Obligation. destruct c; destruct r; simp makeRbtree. Defined.
+  Arguments makeRbtree [c n] _.
+
+  Equations insert c n (t : rbtree c n) : insertResult c n :=
+  insert _ _ t := makeRbtree (ins t).
+
+  Section present.
+    Variable z : nat.
+
+    Lemma present_balance1 : forall n (a : rtree n) (y : nat) c2 (b : rbtree c2 n),
+      present z (projT2 (balance1 a y b))
+      <-> rpresent z a \/ z = y \/ present z b.
+    Proof. intros. funelim (balance1 a y b); simpl in *; tauto. Qed.
+
+    Lemma present_balance2 : forall n (a : rtree n) (y : nat) c2 (b : rbtree c2 n),
+      present z (projT2 (balance2 a y b))
+      <-> rpresent z a \/ z = y \/ present z b.
+    Proof. intros. funelim (balance2 a y b); simpl in *; tauto. Qed.
+
+    Equations present_insResult (c : color) (n : nat) (t : rbtree c n) (r : insResult c n): Prop :=
+    present_insResult Red n t r := rpresent z r <-> z = x \/ present z t;
+    present_insResult Black n t r := present z (projT2 r) <-> z = x \/ present z t.
+
+    Theorem present_ins : forall c n (t : rbtree c n),
+      present_insResult t (ins t).
+    Proof.
+      intros. funelim (ins t); simp present_insResult in *; simpl in *;
+        try match goal with
+          [ |- context [balance1 ?A ?B ?C] ] => generalize (present_balance1 A B C)
+        end;
+        try match goal with
+          [ |- context [balance2 ?A ?B ?C] ] => generalize (present_balance2 A B C)
+        end; tauto.
+    Qed.
+
+    Ltac present_insert t t0 :=
+      intros; funelim (insert t); generalize (present_ins t0);
+      try rewrite present_insResult_equation_1; try rewrite present_insResult_equation_2;
+      funelim (ins t0); intro; assumption.
+
+    Theorem present_insert_Red : forall n (t : rbtree Red n),
+      present z (insert t)
+      <-> (z = x \/ present z t).
+    Proof. present_insert t t0. (* FIXME Qed. *) Admitted.
+
+    Theorem present_insert_Black : forall n (t : rbtree Black n),
+      present z (projT2 (insert t))
+      <-> (z = x \/ present z t).
+    Proof. present_insert t t0. (* FIXME Qed. *) Admitted.
+  End present.
+End insert.
